TestModels/dafny-dependencies/StandardLibrary/src/JavaConversions.dfy
@@ -7,46 +7,49 @@ module StandardLibraryJavaConversions {
   import opened StandardLibrary.Actions
   import opened Wrappers
 
-  class {:extern "java.lang.Void"} Void {
+  class {:compile false} {:extern "java.lang.Void"} Void {
 
   }
 
-  trait {:extern "java.util.function.Consumer"} Consumer<T> {
+  trait {:compile false} {:extern "java.util.function.Consumer"} Consumer<T> {
 
     method {:extern} accept(t: T)
   }
   
-  trait {:extern "java.lang.Throwable"} Throwable {
+  trait {:compile false} {:extern "java.lang.Throwable"} Throwable {
 
   }
 
-  trait {:extern "java.util.concurrent.CompletableFuture"} CompletableFuture<T> {
+  trait {:compile false} {:compile false} {:extern "java.util.concurrent.CompletableFuture"} CompletableFuture<T> {
 
   }
 
-  trait {:extern "org.reactivestreams.Subscription"} Subscription {
+  trait {:compile false} {:extern "org.reactivestreams.Subscription"} Subscription {
 
     method {:extern} request(n: int64)
 
     method {:extern} cancel()
   }
 
-  trait {:extern "software.amazon.awssdk.core.asyn.SdkPublisher"} SdkPublisher<T> {
+  trait {:compile false} {:extern "software.amazon.awssdk.core.asyn.SdkPublisher"} SdkPublisher<T> {
 
     method {:extern} subscribe(s: Subscriber<T>) returns (f: Subscription)
 
   }
 
-  trait {:extern "org.reactivestreams.Subscriber"} Subscriber<T> {
+  trait {:compile false} {:extern "org.reactivestreams.Subscriber"} Subscriber<T> {
 
-    method {:extern} onSubscribe(s: Subscription)
+    // NOTE: Don't put {:extern} on these,
+    // or else no code will be emitted for the implementations.
+
+    method onSubscribe(s: Subscription)
       modifies this
 
-    method {:extern} onNext(t: T)
+    method onNext(t: T)
 
-    method {:extern} onError(t: Throwable)
+    method onError(t: Throwable)
 
-    method {:extern} onComplete()
+    method onComplete()
   }
 
   class SequentialSubscriber<T> extends Subscriber<T> {
@@ -58,23 +61,23 @@ module StandardLibraryJavaConversions {
       this.action := a;
     }
 
-    method {:extern} onSubscribe(s: Subscription) 
+    method onSubscribe(s: Subscription) 
       modifies this
     {
       this.subscription := s;
       subscription.request(1);
     }
 
-    method {:extern} {:verify false} onNext(t: T) {
+    method {:verify false} onNext(t: T) {
       var _ := action.Call(Some(Success(t)));
       subscription.request(1);
     }
 
-    method {:extern} {:verify false} onError(t: Throwable) {
+    method {:verify false} onError(t: Throwable) {
       var _ := action.Call(Some(Failure(t)));
     }
 
-    method {:extern} {:verify false} onComplete() {
+    method {:verify false} onComplete() {
       var _ := action.Call(None);
     }
 
@@ -82,6 +85,41 @@ module StandardLibraryJavaConversions {
 
   method AsSequentialSubscriber<T>(a: Action<StreamEvent<T, Throwable>, ()>) returns (s: Subscriber<T>) {
     s := new SequentialSubscriber(a);
+  }
+
+  // TODO: Rich specification to fill out here.
+  // This could be useful for analysize existing Java codebases to see
+  // if they use ByteBuffers correctly!
+  trait {:compile false} {:extern "java.nio.ByteBuffer"} ByteBuffer {
+    function method {:extern} remaining(): int32
+      ensures remaining() >= 0
+    function method {:extern} position(): int32
+      ensures position() as int + remaining() as int < INT32_MAX_LIMIT
+    function method {:extern} get(i: int32): uint8
+    method {:extern} put(b: uint8)
+
+    static method allocate(capacity: int32) returns (bb: ByteBuffer)
+  }
+
+  method AsBytesRemaining(bb: ByteBuffer) returns (res: seq<uint8>) {
+    // TODO: This is about as efficient as we can get in Dafny code,
+    // but this is a reasonable case to implement in the Java runtime better instead.
+    var length := bb.remaining();
+    var start := bb.position();
+    res := seq(length, (i: nat) requires 0 <= i < length as nat => bb.get(i as int32 + start));
+  }
+
+
+  method ToByteBuffer(b: seq<uint8>) returns (res: ByteBuffer) 
+    requires |b| < INT32_MAX_LIMIT
+  {
+    // TODO: Could do better with native arrays etc.
+    // but this is a reasonable case to implement in the Java runtime better instead.
+    var length := |b| as int32;
+    res := ByteBuffer.allocate(length);
+    for i := 0 to length {
+      res.put(b[i]);
+    }
   }
 
 }
